doc: expand dependent pattern matching support for array literals

src/Init/Data/Array/Basic.lean
@@ -97,8 +97,8 @@ def getOp [Inhabited α] (self : Array α) (idx : Nat) : α :=
 self.get! idx
 
 -- auxiliary declaration used in the equation compiler when pattern matching array literals.
-abbrev getLit {α : Type u} {n : Nat} (a : Array α) (i : Nat) (h₁ : n = a.size) (h₂ : i < n) : α :=
-a.get ⟨i, h₁ ▸ h₂⟩
+abbrev getLit {α : Type u} {n : Nat} (a : Array α) (i : Nat) (h₁ : a.size = n) (h₂ : i < n) : α :=
+a.get ⟨i, h₁.symm ▸ h₂⟩
 
 @[extern "lean_array_fset"]
 def set (a : Array α) (i : @& Fin a.size) (v : α) : Array α :=
