tmp/eqns/matchArrayLit.lean
@@ -1,5 +1,6 @@
-universes u
+universes u v
 
+namespace Experiment1
 inductive ArrayLitMatch (α : Type u)
 | sz0 {}             : ArrayLitMatch
 | sz1 (a₁ : α)       : ArrayLitMatch
@@ -8,13 +9,13 @@ inductive ArrayLitMatch (α : Type u)
 | other {}           : ArrayLitMatch
 
 def matchArrayLit {α : Type u} (a : Array α) : ArrayLitMatch α :=
-if 0 = a.size then
+if a.size = 0 then
   ArrayLitMatch.sz0
-else if h : 1 = a.size then
+else if h : a.size = 1 then
   ArrayLitMatch.sz1 (a.getLit 0 h (ofDecideEqTrue rfl))
-else if h : 2 = a.size then
+else if h : a.size = 2 then
   ArrayLitMatch.sz2 (a.getLit 0 h (ofDecideEqTrue rfl)) (a.getLit 1 h (ofDecideEqTrue rfl))
-else if h : 3 = a.size then
+else if h : a.size = 3 then
   ArrayLitMatch.sz3 (a.getLit 0 h (ofDecideEqTrue rfl)) (a.getLit 1 h (ofDecideEqTrue rfl)) (a.getLit 2 h (ofDecideEqTrue rfl))
 else
   ArrayLitMatch.other
@@ -33,3 +34,176 @@ rfl
 
 def matchArrayLit.eq4 {α : Type u} (a₁ a₂ a₃ a₄ : α) : matchArrayLit #[a₁, a₂, a₃, a₄] = ArrayLitMatch.other :=
 rfl
+end Experiment1
+
+theorem Array.ext {α : Type u} (a b : Array α) : a.size = b.size → (∀ (i : Nat) (hi₁ : i < a.size) (hi₂ : i < b.size) , a.get ⟨i, hi₁⟩ = b.get ⟨i, hi₂⟩) → a = b :=
+match a, b with
+| ⟨sz₁, f₁⟩, ⟨sz₂, f₂⟩ =>
+  show sz₁ = sz₂ → (∀ (i : Nat) (hi₁ : i < sz₁) (hi₂ : i < sz₂) , f₁ ⟨i, hi₁⟩ = f₂ ⟨i, hi₂⟩) → Array.mk sz₁ f₁ = Array.mk sz₂ f₂ from
+  fun h₁ h₂ =>
+    match sz₁, sz₂, f₁, f₂, h₁, h₂ with
+    | sz, _, f₁, f₂, rfl, h₂ =>
+      have f₁ = f₂ from funext $ fun ⟨i, hi₁⟩ => h₂ i hi₁ hi₁;
+      congrArg _ this
+
+theorem Array.extLit {α : Type u} {n : Nat}
+  (a b : Array α)
+  (hsz₁ : a.size = n) (hsz₂ : b.size = n)
+  (h : ∀ (i : Nat) (hi : i < n), a.getLit i hsz₁ hi = b.getLit i hsz₂ hi) : a = b :=
+Array.ext a b (hsz₁.trans hsz₂.symm) $ fun i hi₁ hi₂ => h i (hsz₁ ▸ hi₁)
+
+def toListLitAux {α : Type u} (a : Array α) (n : Nat) (hsz : a.size = n) : ∀ (i : Nat), i ≤ a.size → List α → List α
+| 0,     hi, acc => acc
+| (i+1), hi, acc => toListLitAux i (Nat.leOfSuccLe hi) (a.getLit i hsz (Nat.ltOfLtOfEq (Nat.ltOfLtOfLe (Nat.ltSuccSelf i) hi) hsz) :: acc)
+
+def toArrayLit {α : Type u} (a : Array α) (n : Nat) (hsz : a.size = n) : Array α :=
+List.toArray $ toListLitAux a n hsz n (hsz ▸ Nat.leRefl _) []
+
+theorem toArrayLitEq {α : Type u} (a : Array α) (n : Nat) (hsz : a.size = n) : a = toArrayLit a n hsz :=
+-- TODO: this is painful to prove without proper automation
+sorry
+/-
+First, we need to prove
+∀ i j acc, i ≤ a.size → (toListLitAux a n hsz (i+1) hi acc).index j = if j < i then a.getLit j hsz _ else acc.index (j - i)
+by induction
+
+Base case is trivial
+(j : Nat) (acc : List α) (hi : 0 ≤ a.size)
+     |- (toListLitAux a n hsz 0 hi acc).index j = if j < 0 then a.getLit j hsz _ else acc.index (j - 0)
+...  |- acc.index j = acc.index j
+
+Induction
+
+(j : Nat) (acc : List α) (hi : i+1 ≤ a.size)
+      |- (toListLitAux a n hsz (i+1) hi acc).index j = if j < i + 1 then a.getLit j hsz _ else acc.index (j - (i + 1))
+  ... |- (toListLitAux a n hsz i hi' (a.getLit i hsz _ :: acc)).index j = if j < i + 1 then a.getLit j hsz _ else acc.index (j - (i + 1))  * by def
+  ... |- if j < i     then a.getLit j hsz _ else (a.getLit i hsz _ :: acc).index (j-i)    * by induction hypothesis
+         =
+         if j < i + 1 then a.getLit j hsz _ else acc.index (j - (i + 1))
+If j < i, then both are a.getLit j hsz _
+If j = i, then lhs reduces else-branch to (a.getLit i hsz _) and rhs is then-brachn (a.getLit i hsz _)
+If j >= i + 1, we use
+   - j - i >= 1 > 0
+   - (a::as).index k = as.index (k-1) If k > 0
+   - j - (i + 1) = (j - i) - 1
+   Then lhs = (a.getLit i hsz _ :: acc).index (j-i) = acc.index (j-i-1) = acc.index (j-(i+1)) = rhs
+
+With this proof, we have
+
+∀ j, j < n → (toListLitAux a n hsz n _ []).index j = a.getLit j hsz _
+
+We also need
+
+- (toListLitAux a n hsz n _ []).length = n
+- j < n -> (List.toArray as).getLit j _ _ = as.index j
+
+Then using Array.extLit, we have that a = List.toArray $ toListLitAux a n hsz n _ []
+-/
+
+theorem Array.eqLitOfSize0 {α : Type u} (a : Array α) (hsz : a.size = 0) : a = #[] :=
+toArrayLitEq a 0 hsz
+/-
+Array.ext a #[] h (fun i h₁ h₂ => absurd h₂ (Nat.notLtZero _))
+-/
+
+theorem Array.eqLitOfSize1 {α : Type u} (a : Array α) (hsz : a.size = 1) : a = #[a.getLit 0 hsz (ofDecideEqTrue rfl)] :=
+toArrayLitEq a 1 hsz
+/-
+Array.extLit a #[a.getLit 0 hsz (ofDecideEqTrue rfl)] hsz rfl $ fun i =>
+  match i with
+  | 0     => fun hi => rfl
+  | (n+1) => fun hi =>
+    have n < 0 from hi;
+    absurd this (Nat.notLtZero _)
+-/
+
+theorem Array.eqLitOfSize2 {α : Type u} (a : Array α) (hsz : a.size = 2) : a = #[a.getLit 0 hsz (ofDecideEqTrue rfl), a.getLit 1 hsz (ofDecideEqTrue rfl)] :=
+toArrayLitEq a 2 hsz
+/-
+Array.extLit a #[a.getLit 0 hsz (ofDecideEqTrue rfl), a.getLit 1 hsz (ofDecideEqTrue rfl)] hsz rfl $ fun i =>
+  match i with
+  | 0     => fun hi => rfl
+  | 1     => fun hi => rfl
+  | (n+2) => fun hi =>
+    have n < 0 from hi;
+    absurd this (Nat.notLtZero _)
+-/
+
+theorem Array.eqLitOfSize3 {α : Type u} (a : Array α) (hsz : a.size = 3) :
+  a = #[a.getLit 0 hsz (ofDecideEqTrue rfl), a.getLit 1 hsz (ofDecideEqTrue rfl), a.getLit 2 hsz (ofDecideEqTrue rfl)] :=
+toArrayLitEq a 3 hsz
+/-
+Array.extLit a #[a.getLit 0 hsz (ofDecideEqTrue rfl), a.getLit 1 hsz (ofDecideEqTrue rfl), a.getLit 2 hsz (ofDecideEqTrue rfl)] hsz rfl $ fun i =>
+  match i with
+  | 0     => fun hi => rfl
+  | 1     => fun hi => rfl
+  | 2     => fun hi => rfl
+  | (n+3) => fun hi =>
+    have n < 0 from hi;
+    absurd this (Nat.notLtZero _)
+-/
+
+/-
+Matcher for the following patterns
+```
+| #[]           => _
+| #[a₁]         => _
+| #[a₁, a₂, a₃] => _
+| a             => _
+``` -/
+def matchArrayLit {α : Type u} (C : Array α → Sort v) (a : Array α)
+    (h₁ : Unit →      C #[])
+    (h₂ : ∀ a₁,       C #[a₁])
+    (h₃ : ∀ a₁ a₂ a₃, C #[a₁, a₂, a₃])
+    (h₄ : ∀ a,        C a)
+    : C a :=
+if h : a.size = 0 then
+  @Eq.ndrec _ _ C (h₁ ()) _ (toArrayLitEq a 0 h).symm
+else if h : a.size = 1 then
+  @Eq.ndrec _ _ C (h₂ (a.getLit 0 h (ofDecideEqTrue rfl))) _ (toArrayLitEq a 1 h).symm
+else if h : a.size = 3 then
+  @Eq.ndrec _ _ C (h₃ (a.getLit 0 h (ofDecideEqTrue rfl)) (a.getLit 1 h (ofDecideEqTrue rfl)) (a.getLit 2 h (ofDecideEqTrue rfl))) _ (toArrayLitEq a 3 h).symm
+else
+  h₄ a
+
+/- Equational lemmas that should be generated automatically. -/
+theorem matchArrayLit.eq1 {α : Type u} (C : Array α → Sort v)
+    (h₁ : Unit →      C #[])
+    (h₂ : ∀ a₁,       C #[a₁])
+    (h₃ : ∀ a₁ a₂ a₃, C #[a₁, a₂, a₃])
+    (h₄ : ∀ a,        C a)
+    : matchArrayLit C #[] h₁ h₂ h₃ h₄ = h₁ () :=
+rfl
+
+theorem matchArrayLit.eq2 {α : Type u} (C : Array α → Sort v)
+    (h₁ : Unit →      C #[])
+    (h₂ : ∀ a₁,       C #[a₁])
+    (h₃ : ∀ a₁ a₂ a₃, C #[a₁, a₂, a₃])
+    (h₄ : ∀ a,        C a)
+    (a₁ : α)
+    : matchArrayLit C #[a₁] h₁ h₂ h₃ h₄ = h₂ a₁ :=
+rfl
+
+theorem matchArrayLit.eq3 {α : Type u} (C : Array α → Sort v)
+    (h₁ : Unit →      C #[])
+    (h₂ : ∀ a₁,       C #[a₁])
+    (h₃ : ∀ a₁ a₂ a₃, C #[a₁, a₂, a₃])
+    (h₄ : ∀ a,        C a)
+    (a₁ a₂ a₃ : α)
+    : matchArrayLit C #[a₁, a₂, a₃] h₁ h₂ h₃ h₄ = h₃ a₁ a₂ a₃ :=
+rfl
+
+theorem matchArrayLit.eq4 {α : Type u} (C : Array α → Sort v)
+    (h₁ : Unit →      C #[])
+    (h₂ : ∀ a₁,       C #[a₁])
+    (h₃ : ∀ a₁ a₂ a₃, C #[a₁, a₂, a₃])
+    (h₄ : ∀ a,        C a)
+    (a : Array α)
+    (n₁ : a.size ≠ 0) (n₂ : a.size ≠ 1) (n₃ : a.size ≠ 3)
+    : matchArrayLit C a h₁ h₂ h₃ h₄ = h₄ a :=
+match a, n₁, n₂, n₃ with
+| ⟨0, _⟩,   n₁, _, _  => absurd rfl n₁
+| ⟨1, _⟩,   _,  n₂, _ => absurd rfl n₂
+| ⟨2, _⟩,   _, _, _   => rfl
+| ⟨3, _⟩,   _, _, n₃  => absurd rfl n₃
+| ⟨n+4, _⟩, _, _, _   => rfl
